Separate semantics variant with additional variables out into theory of its own

LaunchburyMoreFree.thy
@@ -1,39 +1,60 @@
-theory Launchbury
-imports Terms Heap
+theory LaunchburyMoreFree
+imports Terms Heap Launchbury
 begin
 
-inductive reds :: "heap \<Rightarrow> exp \<Rightarrow> var list \<Rightarrow> heap \<Rightarrow> exp \<Rightarrow> bool" ("_ : _ \<Down>\<^bsub>_\<^esub> _ : _" [50,50,50,50] 50)
+inductive reds :: "heap \<Rightarrow> exp \<Rightarrow> var list \<Rightarrow> heap \<Rightarrow> exp \<Rightarrow> bool" ("_ : _ \<Down>*\<^bsub>_\<^esub> _ : _" [50,50,50,50] 50)
 where
-  Lambda: "\<Gamma> : (Lam [x]. e) \<Down>\<^bsub>L\<^esub> \<Gamma> : (Lam [x]. e)" 
+  Lambda: "\<Gamma> : (Lam [x]. e) \<Down>*\<^bsub>L\<^esub> \<Gamma> : (Lam [x]. e)" 
  | Application: "\<lbrakk>
-    atom y \<sharp> (\<Gamma>,e,x,L,\<Delta>,\<Theta>,z) ;
-    \<Gamma> : e \<Down>\<^bsub>x#L\<^esub> \<Delta> : (Lam [y]. e');
-    \<Delta> : e'[y ::= x] \<Down>\<^bsub>L\<^esub> \<Theta> : z
+    atom y \<sharp> (\<Gamma>,e,x,L,\<Delta>,\<Theta>,z,n) ;
+    atom (n::var) \<sharp> (\<Gamma>,e,x,L,\<Delta>,\<Theta>,z) ;
+    \<Gamma> : e \<Down>*\<^bsub>n#x#L\<^esub> \<Delta> : (Lam [y]. e');
+    \<Delta> : e'[y ::= x] \<Down>*\<^bsub>L\<^esub> \<Theta> : z
   \<rbrakk>  \<Longrightarrow>
-    \<Gamma> : App e x \<Down>\<^bsub>L\<^esub> \<Theta> : z" 
+    \<Gamma> : App e x \<Down>*\<^bsub>L\<^esub> \<Theta> : z" 
  | Variable: "\<lbrakk>
-    (x,e) \<in> set \<Gamma>; removeAll (x, e) \<Gamma> : e \<Down>\<^bsub>x#L\<^esub> \<Delta> : z \<rbrakk> \<Longrightarrow> \<Gamma> : Var x \<Down>\<^bsub>L\<^esub> (x, z) # \<Delta> : z"
- | Let: "set (bn as) \<sharp>* (\<Gamma>, Let as body, L) \<Longrightarrow> distinctVars (asToHeap as) \<Longrightarrow> asToHeap as @ \<Gamma> : body \<Down>\<^bsub>L\<^esub> \<Delta> : z \<Longrightarrow> \<Gamma> : Let as body \<Down>\<^bsub>L\<^esub> \<Delta> : z"
+    (x,e) \<in> set \<Gamma>; removeAll (x, e) \<Gamma> : e \<Down>*\<^bsub>x#L\<^esub> \<Delta> : z \<rbrakk> \<Longrightarrow> \<Gamma> : Var x \<Down>*\<^bsub>L\<^esub> (x, z) # \<Delta> : z"
+ | Let: "set (bn as) \<sharp>* (\<Gamma>, Let as body, L) \<Longrightarrow> distinctVars (asToHeap as) \<Longrightarrow> asToHeap as @ \<Gamma> : body \<Down>*\<^bsub>L\<^esub> \<Delta> : z \<Longrightarrow> \<Gamma> : Let as body \<Down>*\<^bsub>L\<^esub> \<Delta> : z"
 
 equivariance reds
 
 nominal_inductive reds
-  avoids Application: "y"
+(*
+  avoids LetACons: "v"
+apply (auto simp add: fresh_star_def fresh_Pair exp_assn.fresh exp_assn.bn_defs)
+done
+*)
+  avoids Application: "y" and "n"
 apply (auto simp add: fresh_star_def fresh_Pair exp_assn.fresh)
 done
 
 lemma eval_test:
-  "[] : (Let (ACons x (Lam [y]. Var y) ANil) (Var x)) \<Down>\<^bsub>[]\<^esub> [(x, Lam [y]. Var y)] : (Lam [y]. Var y)"
+  "[] : (Let (ACons x (Lam [y]. Var y) ANil) (Var x)) \<Down>*\<^bsub>[]\<^esub> [(x, Lam [y]. Var y)] : (Lam [y]. Var y)"
 apply(auto intro!: Lambda Application Variable Let
  simp add: fresh_Pair fresh_Cons fresh_Nil exp_assn.fresh fresh_star_def)
 done
 
 lemma eval_test2:
-  "y \<noteq> x \<Longrightarrow> n \<noteq> y \<Longrightarrow> n \<noteq> x \<Longrightarrow>[] : (Let (ACons x (Lam [y]. Var y) ANil) (App (Var x) x)) \<Down>\<^bsub>[]\<^esub> [(x, Lam [y]. Var y)] : (Lam [y]. Var y)"
-  by (auto intro!: Lambda Application Variable Let simp add: fresh_Pair fresh_at_base fresh_Cons fresh_Nil exp_assn.fresh fresh_star_def)
+  "y \<noteq> x \<Longrightarrow> n \<noteq> y \<Longrightarrow> n \<noteq> x \<Longrightarrow>[] : (Let (ACons x (Lam [y]. Var y) ANil) (App (Var x) x)) \<Down>*\<^bsub>[]\<^esub> [(x, Lam [y]. Var y)] : (Lam [y]. Var y)"
+ (* by (auto intro!: Lambda Application Variable Let simp add: fresh_Pair fresh_at_base fresh_Cons fresh_Nil exp_assn.fresh fresh_star_def)*)
+  apply (rule reds.intros)
+  apply (auto simp add: fresh_Pair fresh_at_base fresh_Cons fresh_Nil exp_assn.fresh fresh_star_def)[2]
+  apply (rule Application[where y = y and n = n])
+  prefer 3
+  apply (rule reds.intros)
+  apply simp
+  apply (rule reds.intros)
+  apply (auto simp add: fresh_Pair fresh_at_base fresh_Cons fresh_Nil exp_assn.fresh fresh_star_def)[1]
+  apply (auto simp add: fresh_Pair fresh_at_base fresh_Cons fresh_Nil exp_assn.fresh fresh_star_def)[1]
+  apply simp
+  apply (rule reds.intros)
+  apply simp
+  apply simp
+  apply (rule reds.intros)
+  done
 
 lemma reds_doesnt_forget:
-  "\<Gamma> : e \<Down>\<^bsub>L\<^esub> \<Delta> : z \<Longrightarrow> heapVars \<Gamma> \<subseteq> heapVars \<Delta>"
+  "\<Gamma> : e \<Down>*\<^bsub>L\<^esub> \<Delta> : z \<Longrightarrow> heapVars \<Gamma> \<subseteq> heapVars \<Delta>"
 proof(induct rule: reds.induct)
 case(Variable v e \<Gamma> L \<Delta> z)
   show ?case
@@ -55,7 +76,7 @@ case(Variable v e \<Gamma> L \<Delta> z)
 qed (auto)
 
 lemma reds_avoids_live:
-  "\<lbrakk> \<Gamma> : e \<Down>\<^bsub>L\<^esub> \<Delta> : z;
+  "\<lbrakk> \<Gamma> : e \<Down>*\<^bsub>L\<^esub> \<Delta> : z;
    x \<in> set L;
    x \<notin> heapVars \<Gamma>
   \<rbrakk> \<Longrightarrow> x \<notin> heapVars \<Delta>"
@@ -81,7 +102,7 @@ case (Let as \<Gamma> body L \<Delta> z)
 qed
 
 lemma reds_pres_distinctVars:
-  "\<Gamma> : e \<Down>\<^bsub>L\<^esub> \<Delta> : z \<Longrightarrow> distinctVars \<Gamma> \<Longrightarrow> distinctVars \<Delta>"
+  "\<Gamma> : e \<Down>*\<^bsub>L\<^esub> \<Delta> : z \<Longrightarrow> distinctVars \<Gamma> \<Longrightarrow> distinctVars \<Delta>"
 proof (nominal_induct rule: reds.strong_induct)
   case (Variable x e \<Gamma> L \<Delta> z)
     have "x \<notin> heapVars \<Delta>"
@@ -98,14 +119,14 @@ proof (nominal_induct rule: reds.strong_induct)
 qed (auto intro: distinctVars_append_asToHeap)
 
 
-lemma reds_fresh:" \<lbrakk> \<Gamma> : e \<Down>\<^bsub>L\<^esub> \<Delta> : z;
+lemma reds_fresh:" \<lbrakk> \<Gamma> : e \<Down>*\<^bsub>L\<^esub> \<Delta> : z;
    atom (x::var) \<sharp> (\<Gamma>, e)
   \<rbrakk> \<Longrightarrow> atom x \<sharp> (\<Delta>, z) \<or> x \<in> (heapVars \<Delta> - set L)"
 proof(induct rule: reds.induct)
 case (Lambda \<Gamma> x e) thus ?case by auto
 next
-case (Application y \<Gamma> e x' L \<Delta> \<Theta> z e')
-  hence "atom x \<sharp> (\<Delta>, Lam [y]. e') \<or> x \<in> heapVars \<Delta> - set (x' # L)" by (auto simp add: exp_assn.fresh fresh_Pair)
+case (Application y \<Gamma> e x' L \<Delta> \<Theta> z n e')
+  hence "atom x \<sharp> (\<Delta>, Lam [y]. e') \<or> x \<in> heapVars \<Delta> - set (n # x' # L)" by (auto simp add: exp_assn.fresh fresh_Pair)
 
   thus ?case
   proof
@@ -117,16 +138,16 @@ case (Application y \<Gamma> e x' L \<Delta> \<Theta> z e')
         by (auto simp add:fresh_Pair exp_assn.fresh)
       hence "atom x \<sharp> e'[y ::= x']" using Application.prems
         by (auto intro: subst_pres_fresh[rule_format] simp add: fresh_Pair exp_assn.fresh)
-      thus ?thesis using Application.hyps(5) `atom x \<sharp> (\<Delta>, Lam [y]. e')` by auto
+      thus ?thesis using Application.hyps(6) `atom x \<sharp> (\<Delta>, Lam [y]. e')` by auto
     next
     case True
       hence "atom x \<sharp> e'[y ::= x']" using `atom x \<sharp> (\<Delta>, Lam [y]. e')` Application.prems
         by (auto intro:subst_is_fresh simp add: fresh_Pair exp_assn.fresh)
-      thus ?thesis using Application.hyps(5) `atom x \<sharp> (\<Delta>, Lam [y]. e')` by auto
+      thus ?thesis using Application.hyps(6) `atom x \<sharp> (\<Delta>, Lam [y]. e')` by auto
     qed
   next
-    assume "x \<in> heapVars \<Delta>  - set (x' # L)"
-    thus ?thesis using reds_doesnt_forget[OF Application.hyps(4)] by auto
+    assume "x \<in> heapVars \<Delta>  - set (n # x' # L)"
+    thus ?thesis using reds_doesnt_forget[OF Application.hyps(5)] by auto
   qed
 next
 
@@ -162,45 +183,49 @@ case (Let as \<Gamma> body L \<Delta> z)
     qed
 qed
 
-lemma reds_add_var_L: "\<lbrakk> \<Gamma> : e \<Down>\<^bsub>L\<^esub> \<Delta> : z;
+lemma reds_add_var_L: "\<lbrakk> \<Gamma> : e \<Down>*\<^bsub>L\<^esub> \<Delta> : z;
    atom (x::var) \<sharp> (\<Gamma>, e, \<Delta>, z);
    set L' = insert x (set L)
-  \<rbrakk> \<Longrightarrow> \<Gamma> : e \<Down>\<^bsub>L'\<^esub> \<Delta> : z"
+  \<rbrakk> \<Longrightarrow> \<Gamma> : e \<Down>*\<^bsub>L'\<^esub> \<Delta> : z"
 proof(nominal_induct avoiding : L' rule: reds.strong_induct)
 print_cases
 case (Lambda \<Gamma> x e L L')
   show ?case
     by (rule reds.Lambda)
 next
-case (Application y \<Gamma> e xa L \<Delta> \<Theta> z e' L')
+case (Application y \<Gamma> e xa L \<Delta> \<Theta> z n e' L')
   show ?case
   proof(rule reds.Application)
-    show "atom y \<sharp> (\<Gamma>, e, xa, L', \<Delta>, \<Theta>, z)"
+    show "atom y \<sharp> (\<Gamma>, e, xa, L', \<Delta>, \<Theta>, z, n)"
       using Application
       by (auto simp add: fresh_Pair)
   
+    show "atom n \<sharp> (\<Gamma>, e, xa, L', \<Delta>, \<Theta>, z)"
+      using Application
+      by (auto simp add: fresh_Pair)
+
     have "x \<notin> heapVars \<Theta>"
       using `atom x \<sharp> (\<Gamma>, App e xa, \<Theta>, z)`
       apply (simp add: fresh_Pair)
       by (metis heapVars_not_fresh)
     hence "x \<notin> heapVars \<Delta>"
-      by (metis set_mp reds_doesnt_forget[OF Application.hyps(11)])
+      by (metis set_mp reds_doesnt_forget[OF Application.hyps(20)])
 
     have "atom x \<sharp> (\<Gamma>, e)"
       using `atom x \<sharp> (\<Gamma>, App e xa, \<Theta>, z)`
       by (simp add: fresh_Pair exp_assn.fresh)
-    from reds_fresh[OF Application.hyps(9) this] `x \<notin> heapVars \<Delta>`
+    from reds_fresh[OF Application.hyps(18) this] `x \<notin> heapVars \<Delta>`
     have "atom x \<sharp> (\<Delta>, Lam [y]. e')"
       by auto
     hence "atom x \<sharp> (\<Gamma>, e, \<Delta>, Lam [y]. e')"
       using `atom x \<sharp> (\<Gamma>, App e xa, \<Theta>, z)`
       by (simp add: fresh_Pair exp_assn.fresh)
     moreover
-    have "set (xa # L') = insert x (set (xa # L))"
+    have "set (n # xa # L') = insert x (set (n # xa # L))"
       using `set L' = _` by auto
     ultimately
-    show "\<Gamma> : e \<Down>\<^bsub>xa # L'\<^esub> \<Delta> : Lam [y]. e'"
-      by (rule Application.hyps(10))
+    show "\<Gamma> : e \<Down>*\<^bsub>n # xa # L'\<^esub> \<Delta> : Lam [y]. e'"
+      by (rule Application.hyps(19))
 
     have "atom x \<sharp> (\<Delta>, e'[y::=xa])"
       using `atom x \<sharp> (\<Delta>, Lam [y]. e')` `atom x \<sharp> (\<Gamma>, App e xa, \<Theta>, z)` `atom y \<sharp> xa`
@@ -208,14 +233,14 @@ case (Application y \<Gamma> e xa L \<Delta> \<Theta> z e' L')
       apply (rule subst_pres_fresh[rule_format])
       apply simp
       done
-    from reds_fresh[OF Application.hyps(11) this] `x \<notin> heapVars \<Theta>`
+    from reds_fresh[OF Application.hyps(20) this] `x \<notin> heapVars \<Theta>`
     have "atom x \<sharp> (\<Theta>, z)" by auto
     hence "atom x \<sharp> (\<Delta>, e'[y::=xa], \<Theta>, z)"
       using `atom x \<sharp> (\<Delta>, e'[y::=xa])`
       by (simp add: fresh_Pair)
     then
-    show "\<Delta> : e'[y::=xa] \<Down>\<^bsub>L'\<^esub> \<Theta> : z "
-      by (rule Application.hyps(12)[OF _ `set L' = _`])
+    show "\<Delta> : e'[y::=xa] \<Down>*\<^bsub>L'\<^esub> \<Theta> : z "
+      by (rule Application.hyps(21)[OF _ `set L' = _`])
   qed
 next 
 case (Variable xa e \<Gamma> L \<Delta> z L')
@@ -256,6 +281,45 @@ case (Let as \<Gamma> body L \<Delta> z L')
     by (rule reds.Let[OF _ Let.hyps(4) Let.hyps(6)[OF _ Let.prems(2)]])
 qed
 
+lemma reds_more_free:
+  "\<Gamma> : e \<Down>\<^bsub>L\<^esub> \<Delta> : z \<Longrightarrow> \<Gamma> : e \<Down>*\<^bsub>L\<^esub> \<Delta> : z"
+proof(nominal_induct rule: Launchbury.reds.strong_induct)
+case (Lambda \<Gamma> x e L)
+  show ?case by (rule reds.Lambda)
+next
+case (Application y \<Gamma> e x L \<Delta> \<Theta> z e')
+  obtain n :: var where
+    fresh: "atom n \<sharp> (\<Gamma>, e, x, L, \<Delta>, \<Theta>, z, y, Lam [y]. e')" 
+    by (rule obtain_fresh)
+
+  show ?case
+  proof (rule reds.Application)
+    show "atom y \<sharp> (\<Gamma>, e, x, L, \<Delta>, \<Theta>, z, n)"
+      using Application fresh
+      by (auto simp add: fresh_Pair fresh_at_base)
+    show "atom n \<sharp> (\<Gamma>, e, x, L, \<Delta>, \<Theta>, z)"
+      using fresh
+      by (auto simp add: fresh_Pair fresh_at_base)
+
+    have "\<Gamma> : e \<Down>*\<^bsub>x # L\<^esub> \<Delta> : Lam [y]. e'"
+      by (rule Application.hyps)
+    moreover
+    have "atom n \<sharp> (\<Gamma>, e, \<Delta>, Lam [y]. e')"
+      using fresh by (auto simp add: fresh_Pair)
+    ultimately
+    show "\<Gamma> : e \<Down>*\<^bsub>n # x # L\<^esub> \<Delta> : Lam [y]. e'"
+      by (rule reds_add_var_L, simp)
+
+    show "\<Delta> : e'[y::=x] \<Down>*\<^bsub>L\<^esub> \<Theta> : z"
+      by fact
+  qed
+next
+case Variable
+  thus ?case by (auto intro: reds.intros)
+next
+case (Let as \<Gamma> body L \<Delta> z)
+  thus ?case
+    by (auto intro: reds.Let simp add: fresh_star_Pair)
+qed
 
 end
-
