Launchbury-Unstack.thy
@@ -1,5 +1,5 @@
 theory "Launchbury-Unstack"
-imports Launchbury LaunchburyStacked
+imports Launchbury LaunchburyStacked LaunchburyMoreFree
 begin
 
 lemma supp_set_mem: "x \<in> set L \<Longrightarrow> supp x \<subseteq> supp L"
@@ -10,7 +10,7 @@ lemma forget_stack:
   and "supp S \<subseteq> supp (tl \<Gamma>')"
   shows "\<Gamma> : snd (hd \<Gamma>') \<Down>\<^bsub>S\<^esub> \<Delta> : snd (hd \<Delta>')"
 using assms
-proof (nominal_induct avoiding: S rule: reds.strong_induct)
+proof (nominal_induct avoiding: S rule: LaunchburyStacked.reds.strong_induct)
 case (Lambda \<Gamma> x y e \<Gamma>')
   show ?case
     by (auto intro: Launchbury.reds.intros)
@@ -24,27 +24,14 @@ case (Application n \<Gamma> \<Gamma>' \<Delta> \<Delta>' x e y \<Theta> \<Theta
     using Application stack_not_empty[OF Application(24)]
     by (cases \<Theta>', auto simp add: fresh_Cons fresh_Pair)
   ultimately
-  have fresh: "atom z \<sharp> (\<Gamma>, e, y, S, \<Delta>, \<Theta>, snd (hd \<Theta>'), n)"
+  have fresh: "atom z \<sharp> (\<Gamma>, e, y, S, \<Delta>, \<Theta>, snd (hd \<Theta>'))"
     using Application
     by (simp add: fresh_Pair fresh_Cons fresh_at_base)[1]
 
-  have "atom n \<sharp> \<Gamma>'" using Application by (simp add: fresh_Pair)
-  hence "atom n \<sharp> map fst \<Gamma>'"
-    by (induct \<Gamma>')(auto simp add: fresh_Cons fresh_Nil)
-  moreover
-  have  "atom n \<sharp> snd (hd \<Theta>')"
-    using Application stack_not_empty[OF Application(24)]
-    by (cases \<Theta>', auto simp add: fresh_Cons fresh_Pair)
-  ultimately
-  have fresh2: "atom n \<sharp> (\<Gamma>, e, y, S, \<Delta>, \<Theta>, snd (hd \<Theta>'))"
-    using Application
-    by (simp add: fresh_Pair fresh_Cons fresh_at_base)[1]
- 
-
-  have "supp (n # y # S) \<subseteq> supp ( (x, App (Var n) y) # \<Gamma>')"
+  have "supp (y # S) \<subseteq> supp ( (x, App (Var n) y) # \<Gamma>')"
     using Application.prems(1)
     by (auto simp add: supp_Cons supp_Pair exp_assn.supp)
-  hence hyp1: "\<Gamma> : e \<Down>\<^bsub>n # y # S\<^esub> \<Delta> : Lam [z]. e'" 
+  hence hyp1: "\<Gamma> : e \<Down>\<^bsub>y # S\<^esub> \<Delta> : Lam [z]. e'" 
     by (rule Application.hyps(23)[simplified])
   have "supp S \<subseteq> supp \<Delta>'"
     using Application.prems(1)
@@ -54,7 +41,7 @@ case (Application n \<Gamma> \<Gamma>' \<Delta> \<Delta>' x e y \<Theta> \<Theta
     by (rule Application.hyps(25)[simplified])
    
   show ?case
-    by (simp, rule Launchbury.Application[OF fresh fresh2 hyp1 hyp2])
+    by (simp, rule Launchbury.Application[OF fresh hyp1 hyp2])
 next
 case (Variable y e \<Gamma> x \<Gamma>' \<Delta> z \<Delta>' S)
   have "supp (y # S) \<subseteq> supp ((x, Var y) # \<Gamma>')"
@@ -82,16 +69,16 @@ case (Let as \<Gamma> x body \<Gamma>' \<Delta> \<Delta>' S)
     by (simp, rule Launchbury.Let[OF fresh Let.hyps(5) hyp])
 qed
 
-lemma add_stack:
-  assumes "\<Gamma> : e \<Down>\<^bsub>L\<^esub> \<Delta> : z"
+lemma add_stack_more_fresh:
+  assumes "\<Gamma> : e \<Down>*\<^bsub>L\<^esub> \<Delta> : z"
   assumes "x \<in> set L"
   assumes "supp \<Gamma>' \<subseteq> supp L"
   shows "\<Gamma> : (x,e) # \<Gamma>' \<Down> \<Delta> : (x,z) # \<Gamma>'"
 using assms
-proof (nominal_induct avoiding: \<Gamma>' x rule: Launchbury.reds.strong_induct)
+proof (nominal_induct avoiding: \<Gamma>' x rule: LaunchburyMoreFree.reds.strong_induct)
 case (Lambda \<Gamma> xa e L \<Gamma>')
   show ?case
-    by (auto intro: reds.intros)
+    by (auto intro: LaunchburyStacked.reds.intros)
 next
 case (Application y \<Gamma> e xa L \<Delta> \<Theta> z n e' \<Gamma>' x)
   have fresh_n: "atom n \<sharp> (\<Gamma>, \<Gamma>', \<Delta>, \<Gamma>', x, e, xa, \<Theta>, (x, z) # \<Gamma>', y)"
@@ -115,7 +102,7 @@ case (Application y \<Gamma> e xa L \<Delta> \<Theta> z n e' \<Gamma>' x)
     done
 
   show ?case
-    by (rule reds.Application[OF fresh_n fresh_y hyp1 hyp2])
+    by (rule LaunchburyStacked.reds.Application[OF fresh_n fresh_y hyp1 hyp2])
 next
 case (Variable x e \<Gamma> L \<Delta> z \<Gamma>' xa)
   have "supp ((xa, Var x) # \<Gamma>') \<subseteq> supp (x # L)"
@@ -126,7 +113,7 @@ case (Variable x e \<Gamma> L \<Delta> z \<Gamma>' xa)
     apply (simp)
     done
   show ?case
-    by (rule reds.Variable[OF `(x,e) \<in> set _` hyp])
+    by (rule LaunchburyStacked.reds.Variable[OF `(x,e) \<in> set _` hyp])
 next
 case (Let as \<Gamma> body L \<Delta> z \<Gamma>' x)
   from `x \<in> set L` and `_ \<sharp>* L`
@@ -146,8 +133,16 @@ case (Let as \<Gamma> body L \<Delta> z \<Gamma>' x)
     done
 
   show ?case
-    by (rule reds.Let[OF fresh `distinctVars (asToHeap as)` hyp])
+    by (rule LaunchburyStacked.reds.Let[OF fresh `distinctVars (asToHeap as)` hyp])
 qed
 
+lemma add_stack:
+  assumes "\<Gamma> : e \<Down>\<^bsub>L\<^esub> \<Delta> : z"
+  assumes "x \<in> set L"
+  assumes "supp \<Gamma>' \<subseteq> supp L"
+  shows "\<Gamma> : (x,e) # \<Gamma>' \<Down> \<Delta> : (x,z) # \<Gamma>'"
+  using assms
+  apply (rule add_stack_more_fresh[OF reds_more_free])
+done
 
 end
